---
layout: post
title: Important Formulas for Statistical Mechanics
date: 2024-12-29 15:12:00+0800
description: Statistical Mechanics Notes 
tags: physics formulas
categories: StatisticalMechanics
related_posts: false
---

##### Thermal Wavelemgth
\begin{equation}
\lambda = \frac{h}{\sqrt{2\pi m k_B T}}
\end{equation}
##### Fugacity
\begin{equation}
z = e^{\beta\mu}=e^{\frac{\mu}{k_B T}}
\end{equation}
##### Classical Limit
###### Classical Formulas
\begin{equation}
U = \frac{3}{2} PV
\end{equation}
###### Corrected EOS
\begin{equation}
PV = Nk_B T [1 -\zeta 2^{-5/2} \frac{n\lambda^3}{g}+ \cdots]
\end{equation}

##### Fermi and Bose Functions
\begin{equation}
f_k (z)=\sum_{l=1}^{\infty}(-1)^{l+1}\frac{z^l}{l^k}
\end{equation}
\begin{equation}
g_k (z)=\sum_{l=1}^{\infty}\frac{z^l}{l^k}
\end{equation}

##### Parametric EOS (Important)
For Fermi case:
\begin{equation}
\frac{\lambda^3 P}{k_B T} =g f_{5/2}(z)
\end{equation}
\begin{equation}
\lambda^3 n=g f_{3/2}(z)
\end{equation}
\begin{equation}
U = \frac{3}{2}PV
\end{equation}
For Bose case changing $$f(z)$$ to $$g(z)$$.
##### Fermi and Bose Distribution
\begin{equation}
\bar n_j = \frac{g_j}{e^{-\alpha +\beta\epsilon_j}-\zeta}
\end{equation}
where $$\alpha = \beta\mu$$ and $$\beta = \frac{1}{k_B T}$$.

##### Partition Functions
\begin{equation}
Z_N(V,T) = \sum_s e^{-\beta E_s} Tr(e^{-\beta \hat H})
\end{equation}
\begin{equation}
\Xi (z,V,T) = \sun_{N=0}^{\infty}z^N Z_N(V,T)=Tr(e^{-\beta(\hat H-\mu \hat N)})
\end{equation}
##### Density Operator
\begin{equation}
\hat\rho = \frac{1}{Z}e^{-\beta\hat H}
\end{equation}
\begin{equation}
\hat\rho = \frac{1}{\Xi}e^{-\beta(\hat H-\mu\hat N)}
\end{equation}
##### Von Neumann Entropy
\begin{equation}
S=-Tr(\rho \ln\rho)
\end{equation}
##### Quantum Ideal Gas
###### Grand Partition Function
\begin{equation}
\Xi = \prod_i (1-\zeta e^{-\beta(E_i -\mu)})^{-\zeta}
\end{equation}
###### Average Particle Number
\begin{equation}
\langle N\rangle = \frac{1}{\beta}\frac{\partial \ln \Xi}{\partial \mu}=\sum_{i}\frac{1}{e^{\beta(E_i -\mu)}-\zeta}
\end{equation}
